\begin{array}{ll}
\mathrm{Quadratic\  Equation} & {x=\frac{-b\pm\sqrt{b_{}^{2}-4ac}}{2a}} \\
\mathrm{DisplayQuadratic\  Equation} & \mathrm{x=\frac{-b\pm\sqrt{b_{}^{2}-4ac}}{2a}} \\
\mathrm{Rational\  Function} & {f(x)=\frac{1-x_{}^{2}}{1-x_{}^{3}}} \\
\mathrm{Rational\  Function} & {f(x)=\frac{(1-x_{}^{2})x_{}^{3}}{1-x_{}^{3}}} \\
\mathrm{Rational\  Function} & {f(x)=\frac{(1-x_{}^{2})(x_{}^{3}-5x)}{1-x_{}^{3}}} \\
\mathrm{Parametrize\  Rational\  Function} & {f(x)=\frac{(a_{i}^{}-x_{}^{2})_{}^{5}}{1-x_{}^{3}}} \\
\mathrm{Stacked\  exponents} & {g(z)=e_{}^{-x_{}^{2}}} \\
\mathrm{Stacked\  exponents} & {g(z)=e_{}^{-(z-a)_{}^{2}}} \\
\mathrm{Stacked\  exponents} & {g(z)=e_{}^{-\underset{i=0}{\overset{\infty}{\sum}}z_{i}^{2}}} \\
\mathrm{Stacked\  exponents} & {g(y)=e_{}^{-\underset{i=0}{\overset{\infty}{\sum}}y_{i}^{2}}} \\
\mathrm{Stacked\  exponents} & {g(z)=e_{}^{-\underset{i=0}{\overset{\infty}{\sum}}z_{}^{\frac{2}{a-i}}}} \\
\mathrm{Cross\  Product} & {\frac{x_{1}^{}-x_{2}^{}}{x_{3}^{}-x_{4}^{}}\frac{x_{1}^{}-x_{4}^{}}{x_{2}^{}-x_{3}^{}}} \\
\mathrm{Cross\  Product} & {(\frac{x_{1}^{}-x_{2}^{}}{x_{3}^{}-x_{4}^{}})(\frac{x_{1}^{}-x_{4}^{}}{x_{2}^{}-x_{3}^{}})} \\
\mathrm{Cross\  Product} & {\left( \frac{x_{1}^{}-x_{2}^{}}{x_{3}^{}-x_{4}^{}} \right)\left( \frac{x_{1}^{}-x_{4}^{}}{x_{2}^{}-x_{3}^{}} \right)} \\
\mathrm{Cross\  Product} & \frac{(x_{1}^{}-x_{2}^{})(x_{3}^{}-x_{4}^{})}{(x_{1}^{}-x_{4}^{})(x_{2}^{}-x_{3}^{})} \\
\end{array}
